\documentclass{article}
\usepackage[utf8]{inputenc}
\usepackage{amsmath}
\usepackage{amssymb}
\title{7.5}
\author{r.suhrit2017 }
\date{March 2021}

\begin{document}

\maketitle

\section{Chapter Examples}
\textbf{1. To evaluate:} $$\int \frac{\tan^3 x}{\cos^3 x}$$
Solution:
\begin{gather*}
   \int \frac{\tan^3 x}{\cos^3 x} dx = \int \frac{\sin^3 x}{\cos^6 x}dx
    \\\int \frac{1-\cos^2 x}{\cos^6 x} \sin x\hspace{2mm} dx
    \\\textbf{Substituting u=}\cos x
    \\\int \frac{u^2-1}{u^6}du = \int (u^{-4}-u^{-6}) du = \frac{u^{-3}}{4} +\frac{u^{-5}}{6} \\=\frac{1}{4u^3}+\frac{1}{6u^5}=\frac{\sec^3}{4}+\frac{sec^5}{6}
\end{gather*}
\section{Exercises}
1.
$$\int \cos x (1+\sin^2 x) dx$$
\begin{gather*}
    = \int \cos x (2-\cos^2 x) dx
    \\= \int 2\cos x (2-\cos^2 x) dx
    \\= 2 \int \cos x -\int \cos^3 x dx
    \\= 2 \sin x -\int \cos x (1-\sin^2 x) dx
    \\= 2 \cos x -\int 1-u^2 du
    \\= 2\cos x -\int 1 du +\int u^2 du 
    \\= 2\cos x -u + \frac{u^3}{3}
    \\= 2\cos x -\sin x + \frac{1}{3} \sin^3 x
    \end{gather*}
2. Evaluate:
$$\int (2x^2-1)e^{x^{2}}\hspace{1mm}dx+$$
\begin{gather*}
   \int (2x^2-1)e^{x^{2}} \hspace{1mm}dx
\\ 2x^2e^{x^2}
\end{gather*}
Evaluate:
$$\int \frac{\ln{x}}{x\sqrt{1+(\ln{x})^2}} \hspace{1mm} dx$$
\begin{gather*}
    \int \frac{\ln{x}}{x\sqrt{1+(\ln{x})^2}} \hspace{1mm} dx
    \\= \int \ln{x} \frac{1}{x\sqrt{1+(\ln{x})^2}} \hspace{1mm} dx
    \\=\frac{x\ln{x}-x}{x\sqrt{1+(\ln{x})^2}} - \int \frac{\ln{x}}{x^3\sqrt{1+(\ln x)^2}(1+(\ln{x})^2)}\hspace{1mm} dx
\end{gather*}
Let us now solve for the integral.
\begin{gather*}
    \int \frac{\ln{x}}{x^3\sqrt{1+(\ln x)^2}(1+(\ln{x})^2)}\hspace{1mm} dx
    \\= \int \frac{\ln{x}}{x^3\sqrt{1+(\ln x)^2}(1+(\ln{x})^2)}\hspace{1mm} dx
\end{gather*}
Substituting $u=\frac{1}{x}$, we have,
\begin{gather*}
    \int \frac{u^3}{\sqrt{1+(\ln{\frac{1}{u}})^2}(1+(\ln{\frac{1}{u}})^2)}
\end{gather*}
\section{abe rakh teri maan ki- rakh}
Evaluate: $$\int \frac{x}{(2x+1)^3}\hspace{1mm}dx$$


  $$ \frac{x}{(2x+1)^3}$$
  $$=\frac{A}{2x+1}+\frac{B}{(2x+1)^2}+\frac{C}{(2x+1)^3}$$
   $$\therefore x=A(4x^2+4x+1)+B(2x+1)+C$$
  $$\therefore x=(4A)x^2+(4A+2B)x+A+B+C$$
  $$\therefore 4A=0$$
   $$4A+2B=1$$
   $$A+B+C=0$$
  $$\therefore A=0 B=\frac{1}{2};\hspace{1mm} C=\frac{-1}{2}$$
  $$\therefore\frac{x}{(2x+1)^3}=\frac{1}{2(2x+1)^2}-\frac{1}{2(2x+1)^3}$$
  $$\therefore \int \frac{x}{(2x+1)^3} \hspace{1mm} dx= \frac{1}{2}\int\frac{1}{(2x-1)^2}\hspace{1mm}dx-\frac{1}{2}\int\frac{1}{(2x-1)^3}\hspace{1mm}dx$$
  $$\frac{1}{4}\int u^{-2}\hspace{1mm}du-\frac{1}{4}\int u^{-3}\hspace{1mm}du$$
  $$=\frac{3}{4u^2}-\frac{2}{4u}$$
  $$=\frac{1-4x}{16x^2+16x+4}$$
  
  To solve:
  $$\int \frac{x-1}{x^2-4x+5}\hspace{1mm}dx$$
  Solution:
  \begin{gather*}
      \frac{x-1}{x^2-4x+5}
      \\=\frac{2x+4(x+1)}{(x^2-4x+5)^2}+\int \frac{2x+4}{(x^2-4x+5)^2} \hspace{1mm} dx
  \end{gather*}
  Taking $u=x^2-4x+5$, $du=2x+4\hspace{1mm}dx$. Therefore:
\begin{gather*}
    \int \frac{x-1}{x^2-4x+5}\hspace{1mm}dx=\frac{2x+4(x+1)}{(x^2-4x+5)^2}+\int \frac{du}{u^2}
    \\\frac{2x+4(x+1)}{(x^2-4x+5)^2}-\frac{1}{u}
    \\=\frac{2x+4(x+1)-(x^2-4x+5)}{(x^2-4x+5)^2}
    \\=\frac{x^2+10x-1}{(x^2-4x+5)^2}
\end{gather*}
To solve:
$$\int \frac{x}{x^4+x^2+1} \hspace{1mm} dx$$
Solution:
\begin{gather*}
   \int \frac{x}{x^4+x^2+1} \hspace{1mm} dx
   \\= -\frac{x(4x^2+2x)}{(x^4+x^2+1)^2} - \int \frac{4x^2+2x}{(x^4+x^2+1)^2} \hspace{1mm}{dx}
\end{gather*}
Taking $u=x^4+x^2+1$ we have $du=(4x^2+2x)dx$. Therefore:
\begin{gather*}
\int \frac{x}{x^4+x^2+1} \hspace{1mm} dx
\\=-\frac{x(4x^2+2x)}{(x^4+x^2+1)^2} - \int \frac{du}{u^2}
\\=\frac{1}{u}-\frac{x(4x^2+2x)}{(x^4+x^2+1)^2}
\\=\frac{1}{x^4+x^2+1}-\frac{x(4x^2+2x)}{(x^4+x^2+1)^2}
=\frac{(x^4+x^2+1)-(4x^3+2x^2)}{(x^4+x^2+1)^2}
\\=\frac{x^4-4x^3-x^2+1}{(x^4+x^2+1)^2}
\end{gather*}
\newpage To solve:
$$\int \sin^5 t \cos^4t\hspace{1mm}dt$$
\begin{gather*}
 \int \sin^5 t \cos^4t\hspace{1mm}dt=\int (\sin^2)^2\cos^2 t \sin t \hspace{1mm} dt
 \\=\int (1-\cos^2 t)\cos t \sin t \hspace{1mm} dt
\end{gather*}
Substituting $u=cos t$ we get $du=(sin t)dt$
\begin{gather*}
    \int \sin^5 t \cos^4t\hspace{1mm}dt=\int u(1-u^2)du
   \\ =\int u \hspace{1mm} du -\int u^3 \hspace{1mm} du
   \\ = \frac{u^2}{2}-\frac{u^4}{4}
    \\=\frac{\cos^2t}{2}-\frac{\cos^4t}{4}
\end{gather*}
Evaluate: $$\int \frac{x^3}{\sqrt{1+x^2}}\hspace{1mm} dx$$
For this, we shall substitute $u=1+x^2$. Threfore $du=(2x)dx$ Now,
\begin{gather*}
\int \frac{x^3}{\sqrt{1+x^2}}\hspace{1mm} dx = \int \frac{x^2}{\sqrt{1+x^2}}x\hspace{1mm} dx
\\=\frac{1}{2}\int \frac{u-1}{\sqrt{u}}\hspace{1mm} du
\\=\frac{1}{2}\int u^{\frac{1}{2}}-u^{-\frac{1}{2}}\hspace{1mm} du
\\=\frac{1}{2}\int u^{\frac{1}{2}}\hspace{1mm} du -\frac{1}{2}\int u^{-\frac{1}{2}}\hspace{1mm} du
\\=\frac{1}{2}\frac{2}{3}u^{\frac{3}{2}}-\frac{1}{2}(2) u^{\frac{1}{2}}+C
\\=\frac{1}{3}u^{\frac{3}{2}}- u^{\frac{1}{2}}+C
\\=\frac{\sqrt{x^2+1}^3}{3}-\frac{3\sqrt{x^2+1}}{3}+C
\\=\frac{\sqrt{x^2+1}^3-3\sqrt{x^2+1}}{3}+C
\\=\frac{(x^2-2)\sqrt{x^2+1}}{3}+C
\end{gather*}
To solve: $$\int \frac{dx}{(1-x^2)^{3/2}}\hspace{1mm}dx$$
\begin{gather*}
    \int \frac{dx}{(1-x^2)^{3/2}}=\int (\frac{1}{\sqrt{1-x^2}})^3 \hspace{1mm}{dx}
\end{gather*}
Integrate with respect to $t$: $$\frac{e^{\sqrt{t}}}{\sqrt{t}}$$
Solution: Substituting $\sqrt{t}=u$, $2du=dx(1/\sqrt{t})$
\begin{gather*}
    \therefore \int \frac{e^{\sqrt{t}}}{\sqrt{t}}\hspace{1mm}dt
    \\=2\int e^u \hspace{1mm}du
    \\=2e^u+C
    \\=2e^{\sqrt{t}}+C
\end{gather*}
Integrate with respect to $x$: $$e^{x+e^{x}}$$
Solution
The integral can be rewritten this way:
$$\int e^x\cdot e^{e^{x}}\hspace{1mm}dx$$
Now we substitute $e^x=u$. Therefore $du=(e^x)dx$
Therefore:
\begin{gather*}
   \int e^{x+e^{x}} \hspace{1mm}d=\int e^u\hspace{1mm}du
   \\=e^u+C
   \\=e^{e^x}+C
\end{gather*}
Integrate with respect to x: $$e^2$$
Substituting 2=x
\begin{gather*}
    e^2=e^x
    \\\therefore \int e^2 \hspace{1mm}dx=e^2+C
\end{gather*}
You thought I was that dumb lol look at your face
\\Solution:$$(e^2)x+C$$
Evaluate the integral with respect to x:$$\arctan{\sqrt{x}}$$
Substitute $f(x)=\arctan{\sqrt{x}}$ and $g(x)=1$
Therefore
\begin{gather*}
\int \arctan{\sqrt{x}} \hspace{1mm}dx
\\=x\arctan{\sqrt{x}}-\int \frac{x}{2\sqrt{x}(x+1)} \hspace{1mm}dx
\\=x\arctan{\sqrt{x}}-\frac{1}{2}\int \frac{\sqrt{x}}{x+1}\hspace{1mm}dx
\end{gather*}
Solving the integral term:
Substituting $u=\sqrt{x}$, we have $du=(2\sqrt{x})dx$ Therefore:
\begin{gather*}
\int \frac{\sqrt{x}}{x+1}\hspace{1mm}dx=2\int\frac{u^2}{u^2+1}du
\\=2\int\frac{u^2+1-1}{u^2+1}=2\int1-\frac{1}{u^2+1}du
\\=2u-2\arctan{u}
\\=2\sqrt{x}-2\arctan{\sqrt{x}}
\\=x\arctan{\sqrt{x}}+\arctan{\sqrt{x}}-\sqrt{x}
\end{gather*}
Evaluate the integral with respect to $x$:
$$\frac{\ln{x}}{x\sqrt{1+(\ln{x})^2}}$$
We will substitute $u=1+(\ln{x})^2$ Therefore $du/2=(\ln{x})/x)dx$. Therefore:
\begin{gather*}
\int \frac{\ln{x}}{x\sqrt{1+(\ln{x})^2}}\hspace{1mm}dx=\frac{1}{2}\int u^{-\frac{1}{2}}\hspace{1mm}du
=\frac{1}{2}2u^{\frac{1}{2}}=\sqrt{u}
\\=\sqrt{1+(\ln{x})^2}
\end{gather*}
Evaluate the integral with respect to x:
$$\int^{1}_{0} (1+\sqrt{x})^8 \hspace{1mm}dx$$
For this we substitute $u=\sqrt{x}$. Therefore we have $2du(\sqrt{x})=dx$ Therefore:
\begin{gather*}
\int^{1}_{0} (1+\sqrt{x})^8 \hspace{1mm}dx=2\int^{2}_{1} u(1+u)^8du
\end{gather*}
Solving the antiderivative:
$$\int u(1+u)^8du=\frac{1}{2}u^2(1+u)^8-\int u^2(1+u)^7du$$
Solving the integral:
$$\int u^2(1+u)^7du=\frac{1}{3}u^3(1+u)^7-\frac{7}{3}\int u^3(1+u)^6du$$
Solving the integral:
$$\int u^3(1+u)^6du=\frac{1}{4}u^4(1+u)^6-(1+\frac{1}{2})\int u^4 (1+u)^5du$$
Solving the integral:
$$\int u^4 (1+u)^5du=\frac{1}{5}u^5(1+u)^5-\int u^5(1+u)^4$$
Solving the integral:
$$\int u^5(1+u)^4=\frac{1}{6}u^6(1+u)^4\frac{2}{3}-\int u^6(1+u)^4du$$
Solving the integral:
$$\int u^6(1+u)^4du=\frac{1}{7}u^7(1+u)^4-\frac{4}{7}-\int u^7(1+u)^3$$
Solving the integral:
\begin{gather*}
\int u^7(1+u)^3=\int u^7(1+u^3+3u^2+3u)du
\\=\int u^7du+\int u^{10}du+\int u^9 du+\int u^8 du
\\=\frac{u^8}{8}+\frac{u^{11}}{11}+\frac{u^{10}}{10}+\frac{u^9}{ 9}
\end{gather*}
Now we proceed to substitute the values and simplify the problem:
\begin{gather*}
\int u^6(1+u)^4du=\frac{1}{7}u^7(1+u)^4-\frac{4}{7}-(\frac{u^8}{8}+\frac{u^{11}}{11}+\frac{u^{10}}{10}+\frac{u^9}{ 9})
\\\int u^5(1+u)^4=\frac{1}{6}u^6(1+u)^4\frac{2}{3}-(\frac{1}{7}u^7(1+u)^4-\frac{4}{7}-(\frac{u^8}{8}+\frac{u^{11}}{11}+\frac{u^{10}}{10}+\frac{u^9}{ 9}))
\\\int u^4 (1+u)^5du=\frac{1}{6}u^6(1+u)^4\frac{2}{3}-(\frac{1}{7}u^7(1+u)^4-\frac{4}{7}-(\frac{u^8}{8}+\frac{u^{11}}{11}+\frac{u^{10}}{10}+\frac{u^9}{ 9})))
\\\int u^3(1+u)^6du=\frac{1}{4}u^4(1+u)^6-(\frac{1}{6}u^6(1+u)^4\frac{2}{3}-(\frac{1}{7}u^7(1+u)^4-\frac{4}{7}-(\frac{u^8}{8}+\frac{u^{11}}{11}+\frac{u^{10}}{10}+\frac{u^9}{ 9}))))
\\\int u^2(1+u)^7du\\=\frac{1}{3}u^3(1+u)^7-\frac{7}{3}(\frac{1}{4}u^4(1+u)^6-(\frac{1}{6}u^6(1+u)^4\frac{2}{3}-(\frac{1}{7}u^7(1+u)^4-\frac{4}{7}-(\frac{u^8}{8}+\frac{u^{11}}{11}+\frac{u^{10}}{10}+\frac{u^9}{ 9})))))
\end{gather*}
$$\\\int u(1+u)^8du\\=$$
$$\frac{1}{2}u^2(1+u)^8-(\frac{1}{3}u^3(1+u)^7-\frac{7}{3}(\frac{1}{4}u^4(1+u)^6-(\frac
{1}{6}u^6(1+u)^4\frac{2}{3}-(\frac{1}{7}u^7(1+u)^4-\frac{4}{7}-(\frac{u^8}{8}+\frac{u^{11}}{11}+\frac{u^{10}}{10}+\frac{u^9}{ 9}))))))$$
And now we have solved for the antiderivative. Since we need the complete integral, I am not going to bother simplifying the result stfu.
$$\frac{1}{2}u^2(1+u)^8-(\frac{1}{3}u^3(1+u)^7-\frac{7}{3}(\frac{1}{4}u^4(1+u)^6-(\frac{1}{6}u^6(1+u)^4\frac{2}{3}-(\frac{1}{7}u^7(1+u)^4-\frac{4}{7}-(\frac{u^8}{8}+\frac{u^{11}}{11}+\frac{u^{10}}{10}+\frac{u^9}{ 9}))))))$$ With limits of integration as 2 and 1 is equal to:
$$(\frac{1}{2}2^2(1+2)^8-(\frac{1}{3}2^3(1+2)^7-\frac{7}{3}(\frac{1}{4}2^4(1+2)^6-(\frac{1}{6}2^6(1+2)^4\frac{2}{3}-(\frac{1}{7}2^7(1+2)^4-\frac{4}{7}-(\frac{2^8}{8}+\frac{2^{11}}{11}+\frac{2^{10}}{10}+\frac{2^9}{ 9})))))))-$$$$(\frac{1}{2}1^2(1+1)^8-(\frac{1}{3}1^3(1+1)^7-\frac{7}{3}(\frac{1}{4}1^4(1+1)^6-(\frac{1}{6}1^6(1+1)^4\frac{2}{3}\\-(\frac{1}{7}1^7(1+1)^4-\frac{4}{7}-(\frac{1^8}{8}+\frac{1^{11}}{11}+\frac{1^{10}}{10}+\frac{1^9}{ 9})))))))$$
\end{document}























