\documentclass{article}
\usepackage[utf8]{inputenc}
\usepackage{amsmath}
\usepackage{amssymb}
\title{I will change it stfu}
\author{r.suhrit2017}
\date{March 2021}
\newcommand{\q}[1]{\begin{right}\textit{\textbf{Q#1}}\end{right}}
\begin{document}
\maketitle
\section{abesaaleh}
\begin{gather*}
\sum^{\infty}_{n=1}\frac{n!}{(kn)!}\text{ is convergent if }\lim_{n\to\infty}\frac{(n+1)!}{(k(n+1)!} \cdot \frac{(kn)!}{n!}=0
\\\lim_{n\to\infty}\frac{(n+1)!}{(k(n+1)!} \cdot \frac{(kn)!}{n!}=\lim_{n\to\infty}\frac{(n+1)(kn)!}{(k(n+1))!}
\end{gather*}
And because I am the biggest idiot in the world I forgot about L'Hospital's rule.
\newpage
\begin{gather*}
\sqrt{3}x+y=4
\\x-2y=5\sqrt{3}
\thf 2\sqrt{3}x+2y=8
\\x-2y=5\sqrt{3}
\\\therefore (2\sqrt{3}+1)x=5\sqrt{3}
\\\therefore x=\frac{5\sqrt{3}}{(2\sqrt{3}+1)}
\\=\frac{5\sqrt{3}}{(2\sqrt{3}+1)}\cdot \frac{(2\sqrt{3}-1)}{(2\sqrt{3}-1)}=\frac{30-5\sqrt{3}{11}
\end{gather*}
\end{document}